# ----- RECURRENCE -----
***

![img3](./images/3.png)

no of moves taken to do this is
M(n)

* M(1) = 1
* M(n) =  M(n-1) + 1 + M(n - 1) = 2M(n - 1) + 1 
* here first M(n-1) is moving the disks from a to c and 1 is for moving the last one to b then second M(n-1) for moving all the other disks from c to b.
* now put M(n) in M(n - 1)
* M(n) = 2(2M(n-2) + 1)+1 = 2<sup>2</sup>M(n-2)+(2 + 1)
* M(n) = 2<sup>2</sup>(2M(n-3) + 1)+(2 + 1) = 2<sup>3</sup>M(n-3)+(4 + 2 + 1)
the last term (4+2+1) is (2<sup>2</sup> + 2<sup>1</sup> + 2<sup>0</sup>) or (2<sup>3</sup>-1) so
* M(n) = 2<sup>3</sup>M(n-3)+(2<sup>3</sup>-1) if expanded 3 times
* if expanded k times:
	* M(n) = 2<sup>k</sup>M(n-k)+(2<sup>k</sup>-1)
	If expanded n-1 times:
	* M(n) = 2<sup>n-1</sup>M(n-(n-1))+(2<sup>n-1</sup>-1)
	* M(n) = 2<sup>n-1</sup>M(1)+(2<sup>n-1</sup>-1)
	* M(n) = 2<sup>n-1</sup>+ 2<sup>n-1</sup>-1
	* M(n) = 2<sup>n</sup>-1